simplified proofs a bit

Cslib/Languages/LambdaCalculus/LocallyNameless/Stlc/StrongNorm.lean
@@ -39,15 +39,14 @@ open scoped Term
     3. contains all neutral locally closed terms, and
     4. is closed under top-level β-reduction of the form (λ M) N P₁ … Pₙ → M ^ N P₁ … Pₙ.
 -/
-inductive saturated (S : Set (Term Var)) : Prop where
-| intro : (∀ M ∈ S, LC M) →
-          (∀ M ∈ S, SN M) →
-          (∀ M, neutral M → LC M → M ∈ S) →
+abbrev saturated (S : Set (Term Var)) : Prop :=
+          (∀ M ∈ S, LC M) ∧
+          (∀ M ∈ S, SN M) ∧
+          (∀ M, neutral M → LC M → M ∈ S) ∧
           (∀ M N P, LC N →
                     SN N →
                     multiApp (M ^ N) P ∈ S →
-                      multiApp ((Term.abs M).app N) P ∈ S) →
-            saturated S
+                      multiApp ((Term.abs M).app N) P ∈ S)
 
 /-- The semantic map maps each type to a corresponding saturated set of terms.
     For the strong normalization proof to work, we must ensure that
@@ -56,7 +55,7 @@ inductive saturated (S : Set (Term Var)) : Prop where
     Strong normalization later follows from the fact that terms in saturated
     sets are strongly normalizing.
 -/
-@[simp]
+@[simp, grind]
 def semanticMap (τ : Ty Base) : Set (Term Var) :=
   match τ with
   | Ty.base _ => { t : Term Var | SN t ∧ LC t }
@@ -68,81 +67,52 @@ def semanticMap (τ : Ty Base) : Set (Term Var) :=
 lemma semanticMap_saturated (τ : Ty Base) :
     @saturated Var (semanticMap τ) := by
   induction τ
-  · case base b =>
-      constructor
-      · simp_all
-      · simp_all
-      · simp_all[sn_neutral]
-      · intro M N P lc_N sn_N h_app
-        constructor
-        · simp_all[sn_multiApp]
-        · have H := h_app.2
-          rw[multiApp_lc] at *
-          grind[open_abs_lc]
+  · case base b => grind[sn_multiApp, sn_neutral, multiApp_lc, open_abs_lc]
   · case arrow τ₁ τ₂ ih₁ ih₂ =>
       constructor
       · intro M hM
-        have H := ih₁.3 (.fvar (fresh {})) (.fvar (fresh {})) (.fvar (fresh {}))
+        have H := ih₁.2.2.1 (.fvar (fresh {})) (.fvar (fresh {})) (.fvar (fresh {}))
         specialize (hM (fvar (fresh {})) H)
         apply (ih₂.1) at hM
         cases hM
         assumption
-      · intro M hM
-        apply sn_app_left M (Term.fvar (fresh {}))
+      · constructor
+        · intro M hM
+          apply sn_app_left M (Term.fvar (fresh {})) <;> grind
         · constructor
-        · have H := ih₁.3 (.fvar (fresh {})) (.fvar (fresh {})) (.fvar (fresh {}))
-          specialize (hM (fvar (fresh {})) H)
-          apply ih₂.2 ; assumption
-      · intro M hneut mlc s hs
-        apply ih₂.3
-        · constructor
-          · assumption
-          · apply ih₁.2
-            assumption
-        · constructor
-          · assumption
-          · apply ih₁.1
-            assumption
-      · intro M N P lc_N sn_N h_app s hs
-        apply ih₂.4 M N (s::P)
-        · apply lc_N
-        · apply sn_N
-        · apply h_app
-          assumption
+          · grind
+          · intro M N P lc_N sn_N h_app s hs
+            apply ih₂.2.2.2 M N (s::P) <;> grind
 
 
 
 
 /-- The `entails_context` predicate ensures that each variable in the context
     is mapped to a term in the corresponding semantic map. -/
-def entails_context (E : Term.Env Var) (Γ : Context Var (Ty Base)) :=
+abbrev entails_context (E : Term.Env Var) (Γ : Context Var (Ty Base)) :=
   ∀ {x τ}, ⟨ x, τ ⟩ ∈ Γ → (multiSubst E (Term.fvar x)) ∈ semanticMap τ
 
 /-- The empty context is entailed by any environment. -/
 lemma entails_context_empty {Γ : Context Var (Ty Base)} :
   entails_context [] Γ := by
   intro x τ h_mem
-  rw[multiSubst]
-  apply (semanticMap_saturated τ).3 <;> constructor
+  have Hsat := (@semanticMap_saturated Var Base _ _ τ)
+  grind
 
 omit [HasFresh Var] in
 /-- The `entails_context` predicate is preserved when extending the context
     with a new variable, provided the new variable is fresh and its
     substitution is in the corresponding semantic map. -/
 lemma entails_context_cons (E : Term.Env Var) (Γ : Context Var (Ty Base))
-  (x : Var) (τ : Ty Base) (sub : Term Var) :
-  x ∉ E.dom ∪ E.fv ∪ Γ.dom →
-  sub ∈ semanticMap τ →
-  entails_context E Γ → entails_context (⟨ x, sub ⟩ :: E) (⟨ x, τ ⟩ :: Γ) := by
-  intro h_fresh h_mem h_entails y σ h_mem
+  (x : Var) (τ : Ty Base) (sub : Term Var)
+  (h_fresh : x ∉ E.dom ∪ E.fv ∪ Γ.dom)
+  (h_mem : sub ∈ semanticMap τ) :
+    entails_context E Γ → entails_context (⟨ x, sub ⟩ :: E) (⟨ x, τ ⟩ :: Γ) := by
+  intro h_entails y σ h_mem
   rw[multiSubst]
   rw[entails_context] at h_entails
   cases h_mem
-  · case head =>
-    rw[multiSubst_fvar_fresh]
-    · rw[subst_fvar]
-      simp_all
-    · simp_all
+  · case head       => grind [multiSubst_fvar_fresh]
   · case tail h_mem =>
     specialize (h_entails h_mem)
     rw [subst_fresh]
@@ -153,59 +123,33 @@ lemma entails_context_cons (E : Term.Env Var) (Γ : Context Var (Ty Base))
 
 /-- The `entails` predicate states that a term `t` is
     semantically valid with respect to a context `Γ` and a type `τ` -/
-def entails (Γ : Context Var (Ty Base)) (t : Term Var) (τ : Ty Base) :=
-  ∀ E, env_LC E → (entails_context E Γ) → (multiSubst E t) ∈ semanticMap τ
+abbrev entails (Γ : Context Var (Ty Base)) (t : Term Var) (τ : Ty Base) :=
+    ∀ E, env_LC E → (entails_context E Γ) → (multiSubst E t) ∈ semanticMap τ
 
 /-- The `soundness` lemma states that if a term `t` has type `τ` in context `Γ`,
     then `t` is semantically valid with respect to `Γ` and `τ` -/
 lemma soundness {Γ : Context Var (Ty Base)} {t : Term Var} {τ : Ty Base} :
-  Γ ⊢ t ∶ τ → entails Γ t τ := by
+    Γ ⊢ t ∶ τ → entails Γ t τ := by
   intro derivation_t
   induction derivation_t
-  · case var Γ xσ_mem_Γ =>
-      intro E lc_E hsat
-      apply hsat xσ_mem_Γ
-  · case' abs σ Γ t τ L IH derivation_t =>
+  · case var Γ xσ_mem_Γ => grind
+  · case' abs σ Γ t τ L HL IH =>
+      have sat_semMap_τ := (@semanticMap_saturated Var Base _ _ τ)
+      have sat_semMap_σ := (@semanticMap_saturated Var Base _ _ σ)
       intro E lc_E hsat s hsat_s
+      have ⟨x, Hfresh⟩ :=
+        fresh_exists <| (t.fv ∪ L ∪ E.dom ∪ E.fv ∪ Context.dom Γ ∪ (multiSubst E t).fv)
+      specialize IH x (by simp_all) (⟨x,s⟩ :: E)
       rw[multiSubst_abs]
-      apply (semanticMap_saturated _).4 _ _ []
-      · apply (semanticMap_saturated _).1
-        assumption
-      · apply (semanticMap_saturated _).2
-        assumption
-      · rw[multiApp]
-        set x := fresh (t.fv ∪ L ∪ E.dom ∪ E.fv ∪ Context.dom Γ ∪ (multiSubst E t).fv)
-        have hfresh : x ∉ t.fv ∪ L ∪ E.dom ∪ E.fv ∪ Context.dom Γ  ∪ (multiSubst E t).fv := by
-          apply fresh_notMem
-        have hfreshL : x ∉ L := by simp_all
-        have H1 := derivation_t x hfreshL
-        rw[entails] at H1
-        specialize H1 (⟨x,s⟩ :: E)
-        rw [multiSubst, multiSubst_open_var, ←subst_intro] at H1
-        · apply H1
-          · apply env_LC_cons
-            · apply (semanticMap_saturated _).1
-              assumption
-            · assumption
-          · apply entails_context_cons <;> simp_all
-        · simp_all
-        · apply (semanticMap_saturated σ).1
-          assumption
-        · simp_all
-        · aesop
-  · case app derivation_t derivation_t' IH IH' =>
-      intro E lc_E hsat
-      rw[multiSubst_app]
-      apply IH E lc_E hsat
-      apply IH' E lc_E hsat
+      apply sat_semMap_τ.2.2.2 _ _ [] <;> grind[entails_context_cons, multiSubst_open_var]
+  · case app derivation_t derivation_t' IH IH' => grind[multiSubst_app]
 
 /-- Using soundness and the fact that the empty context
     is entailed by any environment, we can conclude that
     a well-typed term is strongly normalizing. -/
-theorem strong_norm {Γ} {t : Term Var} {τ : Ty Base} (der : Γ ⊢ t ∶ τ) : SN t := by
-  have H := soundness der [] (by grind) entails_context_empty
-  apply (semanticMap_saturated τ).2
-  assumption
+theorem strong_norm {t : Term Var} {τ : Ty Base} (der : Γ ⊢ t ∶ τ) : SN t := by
+  apply (semanticMap_saturated τ).2.1
+  apply (soundness der [] (by grind) entails_context_empty)
 
 end LambdaCalculus.LocallyNameless.Stlc
 
